KeyManagement/AdversarySafety.v
@@ -12,7 +12,8 @@ Require Import
         MapLtac
         Keys
         Tactics
-        Simulation.
+        Simulation
+        AdversaryUniverse.
 
 Require IdealWorld
         RealWorld.
@@ -208,27 +209,6 @@ Section UniverseLemmas.
 
   (* Step user cipher queues ok *)
 
-  Lemma findUserKeys_multi_add_same_keys_idempotent :
-    forall {A} (usrs : honest_users A) u_id1 u_id2 ks1 ks2 cmd1 cmd2 qmsgs1 qmsgs2 mycs1 mycs2,
-        user_keys usrs u_id1 = Some ks1
-      -> user_keys usrs u_id2 = Some ks2
-      -> findUserKeys (usrs $+ (u_id1, {| key_heap := ks1; protocol := cmd1; msg_heap := qmsgs1; c_heap := mycs1 |})
-                           $+ (u_id2, {| key_heap := ks2; protocol := cmd2; msg_heap := qmsgs2; c_heap := mycs2 |})) = findUserKeys usrs.
-  Proof.
-    intros.
-
-    cases (u_id1 ==n u_id2); subst; clean_map_lookups.
-    - rewrite map_add_eq; eauto.
-      autorewrite with find_user_keys; trivial.
-
-    - remember (usrs $+ (u_id1,{| key_heap := ks1; protocol := cmd1; msg_heap := qmsgs1; c_heap := mycs1 |})) as usrs'.
-      (* unfold user_keys in H0. *)
-      (* destruct (usrs $? u_id2); try discriminate. *)
-      (* destruct H0. *)
-      autorewrite with find_user_keys; subst; autorewrite with find_user_keys; trivial.
-      rewrite add_neq_o; unfold user_keys in *; auto.
-  Qed.
-
   Hint Rewrite @findUserKeys_multi_add_same_keys_idempotent
        using (trivial || unfold user_keys; context_map_rewrites; f_equal; trivial) : find_user_keys.
 
@@ -392,21 +372,6 @@ Section UniverseLemmas.
     rewrite orb_diag; trivial.
   Qed.
 
-  Lemma accepted_safe_msg_pattern_honestly_signed :
-    forall {t} (msg : message t) honestk pat,
-      msg_pattern_safe honestk pat
-      -> msg_accepted_by_pattern pat msg
-      -> msg_honestly_signed honestk msg = true.
-  Proof.
-    intros.
-    destruct msg;
-      repeat match goal with
-             | [ H : msg_pattern_safe _ _ |- _] => invert H
-             | [ H : msg_accepted_by_pattern _ _ |- _] => invert H
-             end; simpl; rewrite <- honest_key_honest_keyb; auto.
-  Qed.
-
-  Hint Resolve accepted_safe_msg_pattern_honestly_signed.
 
   Lemma honest_labeled_step_user_cipher_queues_ok :
     forall {A B C} u_id cs cs' lbl (usrs usrs' : honest_users A) (adv adv' : user_data B)
@@ -1092,19 +1057,21 @@ Section SingleAdversarySimulates.
   Section RealWorldLemmas.
     Import RealWorld.
 
-    Hint Resolve
-         honest_cipher_filter_fn_proper
-         honest_cipher_filter_fn_filter_proper
-         honest_cipher_filter_fn_filter_transpose
-         honest_cipher_filter_fn_filter_proper_eq
-         honest_cipher_filter_fn_filter_transpose_eq.
-
     Hint Rewrite @findUserKeys_readd_user_same_keys_idempotent'
          using (trivial || unfold user_keys; context_map_rewrites; f_equal; trivial) : find_user_keys.
     Hint Rewrite @findUserKeys_readd_user_addnl_keys
          using (trivial || unfold user_keys; context_map_rewrites; f_equal; trivial) : find_user_keys.
     Hint Rewrite @findUserKeys_multi_add_same_keys_idempotent
          using (trivial || unfold user_keys; context_map_rewrites; f_equal; trivial) : find_user_keys.
+
+    Hint Extern 1 (_ $+ (?k, _) $? _ = Some _) => clean_map_lookups; trivial.
+
+    Hint Resolve
+         honest_cipher_filter_fn_proper
+         honest_cipher_filter_fn_filter_proper
+         honest_cipher_filter_fn_filter_transpose
+         honest_cipher_filter_fn_filter_proper_eq
+         honest_cipher_filter_fn_filter_transpose_eq.
 
     Lemma univ_components :
       forall {A B} (U__r : universe A B),
@@ -1131,140 +1098,6 @@ Section SingleAdversarySimulates.
       eexists; intuition. eassumption.
     Qed.
 
-    Lemma clean_ciphers_mapsto_iff : forall honestk cs c_id c,
-        MapsTo c_id c (clean_ciphers honestk cs) <-> MapsTo c_id c cs /\ honest_cipher_filter_fn honestk c_id c = true.
-    Proof.
-      intros.
-      apply filter_iff; eauto.
-    Qed.
-
-    Lemma clean_ciphers_keeps_honest_cipher :
-      forall c_id c honestk cs,
-        cs $? c_id = Some c
-        -> honest_cipher_filter_fn honestk c_id c = true
-        -> clean_ciphers honestk cs $? c_id = Some c.
-    Proof.
-      intros.
-      rewrite <- find_mapsto_iff.
-      rewrite <- find_mapsto_iff in H.
-      apply clean_ciphers_mapsto_iff; intuition idtac.
-    Qed.
-
-    Lemma honest_key_not_cleaned :
-      forall cs c_id c honestk k,
-        cs $? c_id = Some c
-        -> k = cipher_signing_key c
-        -> honest_key honestk k
-        -> clean_ciphers honestk cs $? c_id = Some c.
-    Proof.
-      intros.
-      eapply clean_ciphers_keeps_honest_cipher; auto.
-      unfold honest_cipher_filter_fn, cipher_honestly_signed.
-      cases c; subst; rewrite <- honest_key_honest_keyb; eauto.
-    Qed.
-
-    Hint Constructors
-         msg_accepted_by_pattern
-         msg_contains_only_honest_public_keys.
-
-    Hint Extern 1 (_ $+ (?k, _) $? ?k = Some _) => rewrite add_eq_o.
-    Hint Extern 1 (_ $+ (?k, _) $? ?v = _) => rewrite add_neq_o.
-
-    Lemma clean_ciphers_eliminates_dishonest_cipher :
-      forall c_id c honestk cs k,
-        cs $? c_id = Some c
-        -> honest_keyb honestk k = false
-        -> k = cipher_signing_key c
-        -> clean_ciphers honestk cs $? c_id = None.
-    Proof.
-      intros; unfold clean_ciphers, filter.
-      apply P.fold_rec_bis; intros; eauto.
-      cases (honest_cipher_filter_fn honestk k0 e); eauto.
-      cases (c_id ==n k0); subst; eauto.
-      exfalso.
-      rewrite find_mapsto_iff in H2; rewrite H2 in H; invert H.
-      unfold honest_cipher_filter_fn, cipher_honestly_signed, cipher_signing_key in *.
-      cases c;
-        rewrite Heq in H0; invert H0.
-    Qed.
-
-    Hint Resolve clean_ciphers_eliminates_dishonest_cipher clean_ciphers_keeps_honest_cipher.
-
-    Lemma clean_ciphers_keeps_added_honest_cipher :
-      forall c_id c honestk cs,
-        honest_cipher_filter_fn honestk c_id c = true
-        -> ~ In c_id cs
-        -> clean_ciphers honestk (cs $+ (c_id,c)) = clean_ciphers honestk cs $+ (c_id,c).
-    Proof.
-      intros.
-      apply map_eq_Equal; unfold Equal; intros.
-      cases (c_id ==n y); subst; clean_map_lookups; eauto.
-      unfold clean_ciphers, filter; rewrite fold_add; eauto.
-      rewrite H; auto.
-    Qed.
-
-    Lemma clean_ciphers_reduces_or_keeps_same_ciphers :
-      forall c_id c honestk cs,
-        cs $? c_id = Some c
-        -> ( clean_ciphers honestk  cs $? c_id = Some c
-          /\ honest_keyb honestk (cipher_signing_key c) = true)
-        \/ ( clean_ciphers honestk cs $? c_id = None
-          /\ honest_keyb honestk (cipher_signing_key c) = false).
-    Proof.
-      intros.
-      case_eq (honest_keyb honestk (cipher_signing_key c)); intros; eauto.
-      left; intuition idtac.
-      eapply clean_ciphers_keeps_honest_cipher; eauto.
-      unfold honest_cipher_filter_fn, cipher_signing_key in *.
-      cases c; eauto.
-    Qed.
-
-    Lemma clean_ciphers_no_new_ciphers :
-      forall c_id cs honestk,
-        cs $? c_id = None
-        -> clean_ciphers honestk cs $? c_id = None.
-    Proof.
-      intros.
-      unfold clean_ciphers, filter.
-      apply P.fold_rec_bis; intros; eauto.
-      cases (honest_cipher_filter_fn honestk k e); eauto.
-      - case (c_id ==n k); intro; subst; unfold honest_cipher_filter_fn.
-        + rewrite find_mapsto_iff in H0; rewrite H0 in H; invert H.
-        + rewrite add_neq_o; eauto.
-    Qed.
-
-    Hint Resolve clean_ciphers_no_new_ciphers.
-
-    Lemma clean_ciphers_eliminates_added_dishonest_cipher :
-      forall c_id c honestk cs k,
-        cs $? c_id = None
-        -> honest_keyb honestk k = false
-        -> k = cipher_signing_key c
-        -> clean_ciphers honestk cs = clean_ciphers honestk (cs $+ (c_id,c)).
-    Proof.
-      intros.
-      apply map_eq_Equal; unfold Equal; intros.
-      cases (y ==n c_id); subst.
-      - rewrite clean_ciphers_no_new_ciphers; auto.
-        symmetry.
-        eapply clean_ciphers_eliminates_dishonest_cipher; eauto.
-      - unfold clean_ciphers at 2, filter.
-        rewrite fold_add; auto. simpl.
-        unfold honest_cipher_filter_fn at 1.
-        cases c; simpl in *; rewrite H0; trivial.
-    Qed.
-
-    Lemma not_in_ciphers_not_in_cleaned_ciphers :
-      forall c_id cs honestk,
-          ~ In c_id cs
-        -> ~ In c_id (clean_ciphers honestk cs).
-    Proof.
-      intros.
-      rewrite not_find_in_iff in H.
-      apply not_find_in_iff; eauto.
-    Qed.
-
-    Hint Resolve not_in_ciphers_not_in_cleaned_ciphers.
 
     Lemma honest_heap_private_honestk :
       forall {A} k_id ks u_id (usrs : honest_users A),
@@ -1295,226 +1128,13 @@ Section SingleAdversarySimulates.
          honest_key_not_cleaned
          adv_key_not_honestk.
 
-    Lemma dishonest_cipher_cleaned :
-      forall cs  honestk c_id cipherMsg,
-          honest_keyb honestk (cipher_signing_key cipherMsg) = false
-        -> ~ In c_id cs
-        -> clean_ciphers honestk cs = clean_ciphers honestk (cs $+ (c_id, cipherMsg)).
-    Proof.
-      intros.
-      apply map_eq_Equal; unfold Equal; intros.
-
-      case_eq (cs $? y); intros.
-
-      - eapply clean_ciphers_reduces_or_keeps_same_ciphers in H1.
-        destruct H1; destruct H1;
-          rewrite H1;
-          unfold clean_ciphers, filter;
-          rewrite fold_add by auto;
-          symmetry;
-          unfold honest_cipher_filter_fn; cases cipherMsg; simpl in *;
-            rewrite H; simpl; auto.
-
-      - rewrite clean_ciphers_no_new_ciphers; auto.
-        eapply clean_ciphers_no_new_ciphers in H1.
-        unfold clean_ciphers, filter. rewrite fold_add by auto.
-        unfold honest_cipher_filter_fn; cases cipherMsg; simpl in *; rewrite H; eauto.
-    Qed.
-
-    Hint Resolve dishonest_cipher_cleaned.
-
-    Hint Extern 1 (honest_cipher_filter_fn _ _ _ ?c = _) => unfold honest_cipher_filter_fn; cases c.
-
-    Lemma clean_ciphers_added_honest_cipher_not_cleaned :
-      forall honestk cs c_id c k,
-          honest_key honestk k
-        -> k = cipher_signing_key c
-        -> clean_ciphers honestk (cs $+ (c_id,c)) = clean_ciphers honestk cs $+ (c_id,c).
-    Proof.
-      intros.
-      apply map_eq_Equal; unfold Equal; intros.
-      (* unfold honest_signing_key,honest_key in H. *)
-
-      case (y ==n c_id); intros; subst; clean_map_lookups.
-      - erewrite clean_ciphers_keeps_honest_cipher; auto.
-        invert H; unfold honest_cipher_filter_fn; eauto.
-        unfold cipher_honestly_signed, honest_keyb;
-          cases c; simpl in *; context_map_rewrites; auto.
-      - case_eq (clean_ciphers honestk cs $? y); intros; subst.
-        + cases (cs $? y); subst; eauto.
-          * assert (cs $? y = Some c1) by assumption;
-              eapply clean_ciphers_reduces_or_keeps_same_ciphers in Heq; split_ors;
-                split_ands; subst; contra_map_lookup.
-            eapply clean_ciphers_keeps_honest_cipher; auto.
-            unfold honest_cipher_filter_fn, cipher_honestly_signed;
-              cases c1; simpl in *; auto.
-          * exfalso; eapply clean_ciphers_no_new_ciphers in Heq; contra_map_lookup.
-        + case_eq (cs $? y); intros; subst; eauto.
-          eapply clean_ciphers_eliminates_dishonest_cipher; eauto.
-          case_eq (honest_keyb honestk (cipher_signing_key c0)); intros; subst; auto.
-          exfalso; eapply clean_ciphers_keeps_honest_cipher in H1; contra_map_lookup; auto.
-          unfold honest_cipher_filter_fn, cipher_honestly_signed;
-            cases c0; simpl in *; auto.
-    Qed.
-
-    Lemma clean_ciphers_idempotent :
-      forall uks cs,
-        ciphers_honestly_signed uks cs
-      -> clean_ciphers uks cs = cs.
-    Proof.
-      unfold clean_ciphers, filter, ciphers_honestly_signed; intros.
-      apply P.fold_rec_bis; intros; Equal_eq; subst; eauto.
-      unfold honest_cipher_filter_fn.
-      rewrite find_mapsto_iff in H0.
-      assert (cipher_honestly_signed uks e = true).
-        eapply Forall_natmap_in_prop with (P := fun c => cipher_honestly_signed uks c = true); eauto.
-      rewrite H2; trivial.
-    Qed.
-
-    Lemma clean_ciphers_honestly_signed :
-      forall uks cs,
-        ciphers_honestly_signed uks (clean_ciphers uks cs).
-    Proof.
-      unfold ciphers_honestly_signed; intros.
-      rewrite Forall_natmap_forall; intros.
-      rewrite <- find_mapsto_iff, clean_ciphers_mapsto_iff in H; split_ands.
-      unfold honest_cipher_filter_fn in *; assumption.
-    Qed.
-
-    Lemma clean_messages_keeps_honestly_signed :
-      forall {t} (msg : message t) msgs honestk,
-        msg_honestly_signed honestk msg = true
-        -> clean_messages honestk (msgs ++ [existT _ _ msg])
-          = clean_messages honestk msgs ++ [existT _ _ msg].
-    Proof.
-      intros; unfold clean_messages.
-      induction msgs; simpl; eauto.
-      - rewrite H; trivial.
-      - cases (msg_filter honestk a); subst; eauto.
-        rewrite IHmsgs; trivial.
-    Qed.
-
-    Lemma clean_messages_drops_not_honestly_signed :
-      forall {t} (msg : message t) msgs honestk,
-        msg_honestly_signed honestk msg = false
-        -> clean_messages honestk (msgs ++ [existT _ _ msg])
-          = clean_messages honestk msgs.
-    Proof.
-      intros; unfold clean_messages.
-      induction msgs; simpl; eauto.
-      - rewrite H; trivial.
-      - cases (msg_filter honestk a); subst; eauto.
-        rewrite IHmsgs; trivial.
-    Qed.
-
     Hint Extern 1 (honest_keyb _ _ = true) => rewrite <- honest_key_honest_keyb.
     Hint Extern 1 (_ && _ = true) => rewrite andb_true_iff.
-
-    Lemma clean_message_keeps_safely_patterned_message :
-      forall {t} (msg : message t) honestk msgs pat,
-        msg_pattern_safe honestk pat
-        -> msg_accepted_by_pattern pat msg
-        -> clean_messages honestk (existT _ _ msg :: msgs)
-          = (existT _ _ msg) :: clean_messages honestk msgs.
-    Proof.
-      intros.
-      assert (msg_honestly_signed honestk msg = true) by eauto.
-      unfold clean_messages; simpl;
-        match goal with
-        | [ H : msg_honestly_signed _ _ = _ |- _ ] => rewrite H
-        end; trivial.
-    Qed.
-
-    Lemma clean_messages_idempotent :
-      forall msgs honestk,
-        clean_messages honestk (clean_messages honestk msgs) = clean_messages honestk msgs.
-    Proof.
-      induction msgs; intros; eauto.
-      simpl.
-      case_eq (msg_filter honestk a); intros; eauto.
-      simpl; rewrite H; auto.
-      rewrite IHmsgs; trivial.
-    Qed.
 
     Hint Resolve findUserKeys_foldfn_proper findUserKeys_foldfn_transpose
          findUserKeys_foldfn_proper_Equal findUserKeys_foldfn_transpose_Equal.
 
-    Lemma clean_users_cleans_user :
-      forall {A} (usrs : honest_users A) honestk u_id u_d u_d',
-        usrs $? u_id = Some u_d
-        -> u_d' = {| key_heap := u_d.(key_heap)
-                  ; protocol := u_d.(protocol)
-                  ; msg_heap :=  clean_messages honestk u_d.(msg_heap)
-                  ; c_heap   := u_d.(c_heap) |}
-        -> clean_users honestk usrs $? u_id = Some u_d'.
-    Proof.
-      intros.
-      unfold clean_users; rewrite map_o; unfold option_map;
-        context_map_rewrites; subst; auto.
-    Qed.
 
-    Lemma clean_users_cleans_user_inv :
-      forall {A} (usrs : honest_users A) honestk u_id u_d,
-        clean_users honestk usrs $? u_id = Some u_d
-        -> exists msgs, usrs $? u_id = Some {| key_heap := u_d.(key_heap)
-                                       ; protocol := u_d.(protocol)
-                                       ; msg_heap := msgs
-                                       ; c_heap   := u_d.(c_heap) |}
-                  /\ u_d.(msg_heap) = clean_messages honestk msgs.
-    Proof.
-      intros.
-      unfold clean_users in *. rewrite map_o in H. unfold option_map in *.
-      cases (usrs $? u_id); try discriminate; eauto.
-      destruct u; destruct u_d; simpl in *.
-      invert H.
-      eexists; eauto.
-    Qed.
-
-    Lemma clean_users_add_pull :
-      forall {A} (usrs : honest_users A) honestk u_id u,
-        clean_users honestk (usrs $+ (u_id,u))
-          = clean_users honestk usrs $+ (u_id, {| key_heap := u.(key_heap)
-                                                ; protocol := u.(protocol)
-                                                ; msg_heap :=  clean_messages honestk u.(msg_heap)
-                                                ; c_heap   := u.(c_heap) |}).
-    Proof.
-      intros.
-      apply map_eq_Equal; unfold Equal; intros.
-      cases (y ==n u_id); subst; clean_map_lookups; eauto;
-        unfold clean_users; rewrite !map_o; unfold option_map; clean_map_lookups; auto.
-    Qed.
-
-    Lemma clean_users_no_change_findUserKeys :
-      forall {A} (usrs : honest_users A) honestk,
-        findUserKeys (clean_users honestk usrs) = findUserKeys usrs.
-    Proof.
-      induction usrs using P.map_induction_bis; intros; Equal_eq; contra_map_lookup; auto.
-      unfold findUserKeys.
-      rewrite fold_add; auto.
-      rewrite clean_users_add_pull; auto. simpl.
-      apply map_eq_Equal; unfold Equal; intros.
-      rewrite !fold_add; auto. simpl.
-      rewrite !findUserKeys_notation, IHusrs; trivial.
-
-      unfold not; intros.
-      apply map_in_iff in H0; contradiction.
-    Qed.
-
-    Lemma clean_users_idempotent :
-      forall {A} (usrs : honest_users A) honestk,
-        clean_users honestk (clean_users honestk usrs) = clean_users honestk usrs.
-    Proof.
-      intros; apply map_eq_Equal; unfold Equal; intros.
-      case_eq (clean_users honestk usrs $? y); intros.
-      - destruct u; simpl in *; eapply clean_users_cleans_user; eauto; simpl.
-        apply clean_users_cleans_user_inv in H.
-        destruct H; split_ands; simpl in *; eauto.
-        f_equal; subst; eauto using clean_messages_idempotent.
-      - unfold clean_users in *.
-        rewrite map_o in H; unfold option_map in H; cases (usrs $? y); try discriminate.
-
-        rewrite !map_o, Heq; trivial.
-    Qed.
 
     Lemma user_cipher_queue_cleaned_users_nochange :
       forall {A} (usrs : honest_users A) honestk u_id,
@@ -1583,6 +1203,8 @@ Section SingleAdversarySimulates.
             rewrite <- find_mapsto_iff; eauto.
     Qed.
 
+    Hint Resolve clean_ciphers_keeps_honest_cipher.
+
     Lemma msgCiphersSigned_after_clean_ciphers' :
       forall msgs honestk cs,
         Forall (msgCipherOk honestk cs) msgs
@@ -1593,8 +1215,7 @@ Section SingleAdversarySimulates.
       destruct x; intuition idtac.
       destruct m; eauto.
       repeat match goal with [H : exists _, _ |- _] => destruct H end.
-      repeat eexists.
-      eapply clean_ciphers_keeps_honest_cipher; eauto.
+      repeat eexists; eauto.
     Qed.
 
     Lemma msgCiphersSigned_after_clean_ciphers :
@@ -1707,7 +1328,8 @@ Section SingleAdversarySimulates.
          clean_ciphers_added_honest_cipher_not_cleaned
          findUserKeys_readd_user_same_key_heap_idempotent
          ciphers_honestly_signed_after_msg_keys
-         findUserKeys_has_private_key_of_user.
+         findUserKeys_has_private_key_of_user
+         not_in_ciphers_not_in_cleaned_ciphers.
 
     Lemma cipher_message_keys_already_in_honest :
       forall {A t} (msg : message t) (usrs : honest_users A) honestk cs c_id k__s k__e,
@@ -1815,23 +1437,16 @@ Section SingleAdversarySimulates.
 
       - left.
         autorewrite with find_user_keys.
-        (* erewrite findUserKeys_readd_user_addnl_keys; eauto. *)
-        eapply Forall_natmap_in_prop in H14; eauto.
         assert (findUserKeys usrs' $? k__encid = Some true) by eauto.
-        invert H14; try contradiction.
+        encrypted_ciphers_prop.
         + exfalso; unfold not in *.
-          eapply Forall_natmap_in_prop in H23; eauto.
-          simpl in H23; unfold user_cipher_queue_ok in H23; rewrite Forall_forall in H23; specialize (H23 _ H8).
-          invert H23; split_ands; clean_map_lookups.
-          simpl in *.
-          eapply honest_keyb_true_findKeys in H6; auto.
+          user_cipher_queues_prop.
+          contradiction.
 
         + rewrite merge_keys_mine; eauto; econstructor; eauto.
 
       - left; econstructor; eauto.
-        eapply Forall_natmap_in_prop in H17; eauto.
-        simpl in H17; unfold user_cipher_queue_ok in H17; rewrite Forall_forall in H17; specialize (H17 _ H2).
-        invert H17; split_ands; clean_map_lookups; eauto.
+        user_cipher_queues_prop; eauto.
     Qed.
 
     Lemma honest_cipher_filter_fn_nochange_pubk :
@@ -1946,7 +1561,7 @@ Section SingleAdversarySimulates.
 
         eapply map_eq_Equal; unfold Equal; intros.
         cases (u_id ==n y); subst; clean_map_lookups.
-        + erewrite clean_users_cleans_user; eauto. simpl.
+        + erewrite clean_users_cleans_user; clean_map_lookups; eauto. simpl.
           f_equal.
           rewrite clean_messages_nochange_pubk; auto.
         + unfold clean_users.
@@ -1961,7 +1576,7 @@ Section SingleAdversarySimulates.
 
         eapply map_eq_Equal; unfold Equal; intros.
         cases (y ==n u_id); subst; clean_map_lookups.
-        * erewrite clean_users_cleans_user; eauto.
+        * erewrite clean_users_cleans_user; clean_map_lookups; eauto.
         * unfold clean_users; rewrite !map_o; clean_map_lookups; trivial.
     Qed.
 
@@ -2400,6 +2015,8 @@ Section SingleAdversarySimulates.
         rewrite H6.
         f_equal.
     Qed.
+
+    Hint Resolve dishonest_cipher_cleaned.
 
     Lemma adv_step_implies_no_new_ciphers_after_cleaning :
       forall {A B C} cs cs' lbl (usrs usrs' : honest_users A) (adv adv' : user_data B)
