KeyManagement/AdversaryUniverse.v
@@ -1,0 +1,549 @@
+From Coq Require Import
+     List
+     Morphisms
+     Eqdep
+     (* Program.Equality (* for dependent induction *) *)
+.
+
+Require Import
+        MyPrelude
+        Maps
+        Common
+        MapLtac
+        Keys
+        Tactics.
+
+Require IdealWorld
+        RealWorld.
+
+Set Implicit Arguments.
+
+Lemma accepted_safe_msg_pattern_honestly_signed :
+  forall {t} (msg : RealWorld.message t) honestk pat,
+    RealWorld.msg_pattern_safe honestk pat
+    -> RealWorld.msg_accepted_by_pattern pat msg
+    -> RealWorld.msg_honestly_signed honestk msg = true.
+Proof.
+  intros.
+  destruct msg;
+    repeat match goal with
+           | [ H : RealWorld.msg_pattern_safe _ _ |- _] => invert H
+           | [ H : RealWorld.msg_accepted_by_pattern _ _ |- _] => invert H
+           end; simpl; rewrite <- RealWorld.honest_key_honest_keyb; auto.
+Qed.
+
+Hint Resolve accepted_safe_msg_pattern_honestly_signed.
+
+(******************** CIPHER CLEANING *********************
+ **********************************************************
+ *
+ * Function to clean ciphehrs and lemmas about it.
+ *)
+
+Section CleanCiphers.
+  Import RealWorld.
+
+  Variable honestk : key_perms.
+
+  Definition honest_cipher_filter_fn (c_id : cipher_id) (c : cipher) :=
+    cipher_honestly_signed honestk c.
+
+  Lemma honest_cipher_filter_fn_proper :
+    Proper (eq  ==>  eq  ==>  eq) honest_cipher_filter_fn.
+  Proof.
+    unfold Proper, Morphisms.respectful; intros; subst; reflexivity.
+  Qed.
+
+  Lemma honest_cipher_filter_fn_filter_proper :
+    Proper
+      ( eq  ==>  eq  ==>  Equal  ==>  Equal)
+      (fun (k : NatMap.key) (e : cipher) (m : t cipher) => if honest_cipher_filter_fn k e then m $+ (k, e) else m).
+  Proof.
+    unfold Proper, respectful;
+      unfold Equal; intros; apply map_eq_Equal in H1; subst; auto.
+  Qed.
+
+  Lemma honest_cipher_filter_fn_filter_transpose :
+    transpose_neqkey Equal
+       (fun (k : NatMap.key) (e : cipher) (m : t cipher) => if honest_cipher_filter_fn k e then m $+ (k, e) else m).
+  Proof.
+    unfold transpose_neqkey, Equal, honest_cipher_filter_fn, cipher_honestly_signed; intros.
+    cases e; cases e'; simpl;
+      repeat match goal with
+             | [ |- context[if ?cond then _ else _] ] => cases cond
+             | [ |- context[_ $+ (?k1,_) $? ?k2] ] => cases (k1 ==n k2); subst; clean_map_lookups
+             end; eauto.
+  Qed.
+
+  Lemma honest_cipher_filter_fn_filter_proper_eq :
+    Proper
+      ( eq  ==>  eq  ==>  eq  ==>  eq)
+      (fun (k : NatMap.key) (e : cipher) (m : t cipher) => if honest_cipher_filter_fn k e then m $+ (k, e) else m).
+  Proof.
+    unfold Proper, respectful; intros; subst; trivial.
+  Qed.
+
+  Lemma honest_cipher_filter_fn_filter_transpose_eq :
+    transpose_neqkey eq
+       (fun (k : NatMap.key) (e : cipher) (m : t cipher) => if honest_cipher_filter_fn k e then m $+ (k, e) else m).
+  Proof.
+    unfold transpose_neqkey, honest_cipher_filter_fn, cipher_honestly_signed; intros.
+    cases e; cases e'; subst; simpl;
+      repeat match goal with
+             | [ |- context[if ?cond then _ else _] ] => cases cond
+             | [ |- context[_ $+ (?k1,_) $? ?k2] ] => cases (k1 ==n k2); subst; clean_map_lookups
+             end; eauto;
+        rewrite map_ne_swap; eauto.
+  Qed.
+
+  Definition clean_ciphers (cs : ciphers) :=
+    filter honest_cipher_filter_fn cs.
+
+  Hint Resolve
+       honest_cipher_filter_fn_proper
+       honest_cipher_filter_fn_filter_proper
+       honest_cipher_filter_fn_filter_transpose
+       honest_cipher_filter_fn_filter_proper_eq
+       honest_cipher_filter_fn_filter_transpose_eq.
+
+  Hint Rewrite @findUserKeys_readd_user_same_keys_idempotent'
+       using (trivial || unfold user_keys; context_map_rewrites; f_equal; trivial) : find_user_keys.
+  Hint Rewrite @findUserKeys_readd_user_addnl_keys
+       using (trivial || unfold user_keys; context_map_rewrites; f_equal; trivial) : find_user_keys.
+
+  Lemma findUserKeys_multi_add_same_keys_idempotent :
+    forall {A} (usrs : honest_users A) u_id1 u_id2 ks1 ks2 cmd1 cmd2 qmsgs1 qmsgs2 mycs1 mycs2,
+      user_keys usrs u_id1 = Some ks1
+      -> user_keys usrs u_id2 = Some ks2
+      -> findUserKeys (usrs $+ (u_id1, {| key_heap := ks1; protocol := cmd1; msg_heap := qmsgs1; c_heap := mycs1 |})
+                           $+ (u_id2, {| key_heap := ks2; protocol := cmd2; msg_heap := qmsgs2; c_heap := mycs2 |})) = findUserKeys usrs.
+  Proof.
+    intros.
+
+    cases (u_id1 ==n u_id2); subst; clean_map_lookups.
+    - rewrite map_add_eq; eauto.
+      autorewrite with find_user_keys; trivial.
+
+    - remember (usrs $+ (u_id1,{| key_heap := ks1; protocol := cmd1; msg_heap := qmsgs1; c_heap := mycs1 |})) as usrs'.
+      (* unfold user_keys in H0. *)
+      (* destruct (usrs $? u_id2); try discriminate. *)
+      (* destruct H0. *)
+      autorewrite with find_user_keys; subst; autorewrite with find_user_keys; trivial.
+      rewrite add_neq_o; unfold user_keys in *; auto.
+  Qed.
+
+  Hint Rewrite @findUserKeys_multi_add_same_keys_idempotent
+       using (trivial || unfold user_keys; context_map_rewrites; f_equal; trivial) : find_user_keys.
+
+  Lemma clean_ciphers_mapsto_iff : forall cs c_id c,
+      MapsTo c_id c (clean_ciphers cs) <-> MapsTo c_id c cs /\ honest_cipher_filter_fn c_id c = true.
+  Proof.
+    intros.
+    apply filter_iff; eauto.
+  Qed.
+
+  Lemma clean_ciphers_keeps_honest_cipher :
+    forall c_id c cs,
+      cs $? c_id = Some c
+      -> honest_cipher_filter_fn c_id c = true
+      -> clean_ciphers cs $? c_id = Some c.
+  Proof.
+    intros.
+    rewrite <- find_mapsto_iff.
+    rewrite <- find_mapsto_iff in H.
+    apply clean_ciphers_mapsto_iff; intuition idtac.
+  Qed.
+
+  Lemma honest_key_not_cleaned :
+    forall cs c_id c k,
+      cs $? c_id = Some c
+      -> k = cipher_signing_key c
+      -> honest_key honestk k
+      -> clean_ciphers cs $? c_id = Some c.
+  Proof.
+    intros.
+    eapply clean_ciphers_keeps_honest_cipher; auto.
+    unfold honest_cipher_filter_fn, cipher_honestly_signed.
+    cases c; subst; rewrite <- honest_key_honest_keyb; eauto.
+  Qed.
+
+  Hint Constructors
+       msg_accepted_by_pattern
+       msg_contains_only_honest_public_keys.
+
+  Hint Extern 1 (_ $+ (?k, _) $? ?k = Some _) => rewrite add_eq_o.
+  Hint Extern 1 (_ $+ (?k, _) $? ?v = _) => rewrite add_neq_o.
+
+  Lemma clean_ciphers_eliminates_dishonest_cipher :
+    forall c_id c cs k,
+      cs $? c_id = Some c
+      -> honest_keyb honestk k = false
+      -> k = cipher_signing_key c
+      -> clean_ciphers cs $? c_id = None.
+  Proof.
+    intros; unfold clean_ciphers, filter.
+    apply P.fold_rec_bis; intros; eauto.
+    cases (honest_cipher_filter_fn k0 e); eauto.
+    cases (c_id ==n k0); subst; eauto.
+    exfalso.
+    rewrite find_mapsto_iff in H2; rewrite H2 in H; invert H.
+    unfold honest_cipher_filter_fn, cipher_honestly_signed, cipher_signing_key in *.
+    cases c;
+      rewrite Heq in H0; invert H0.
+  Qed.
+
+  Hint Resolve clean_ciphers_eliminates_dishonest_cipher clean_ciphers_keeps_honest_cipher.
+
+  Lemma clean_ciphers_keeps_added_honest_cipher :
+    forall c_id c cs,
+      honest_cipher_filter_fn c_id c = true
+      -> ~ In c_id cs
+      -> clean_ciphers (cs $+ (c_id,c)) = clean_ciphers cs $+ (c_id,c).
+  Proof.
+    intros.
+    apply map_eq_Equal; unfold Equal; intros.
+    cases (c_id ==n y); subst; clean_map_lookups; eauto.
+    unfold clean_ciphers, filter; rewrite fold_add; eauto.
+    rewrite H; auto.
+  Qed.
+
+  Lemma clean_ciphers_reduces_or_keeps_same_ciphers :
+    forall c_id c cs,
+      cs $? c_id = Some c
+      -> ( clean_ciphers  cs $? c_id = Some c
+        /\ honest_keyb honestk (cipher_signing_key c) = true)
+      \/ ( clean_ciphers cs $? c_id = None
+        /\ honest_keyb honestk (cipher_signing_key c) = false).
+  Proof.
+    intros.
+    case_eq (honest_keyb honestk (cipher_signing_key c)); intros; eauto.
+    left; intuition idtac.
+    eapply clean_ciphers_keeps_honest_cipher; eauto.
+    unfold honest_cipher_filter_fn, cipher_signing_key in *.
+    cases c; eauto.
+  Qed.
+
+  Lemma clean_ciphers_no_new_ciphers :
+    forall c_id cs,
+      cs $? c_id = None
+      -> clean_ciphers cs $? c_id = None.
+  Proof.
+    intros.
+    unfold clean_ciphers, filter.
+    apply P.fold_rec_bis; intros; eauto.
+    cases (honest_cipher_filter_fn k e); eauto.
+    - case (c_id ==n k); intro; subst; unfold honest_cipher_filter_fn.
+      + rewrite find_mapsto_iff in H0; rewrite H0 in H; invert H.
+      + rewrite add_neq_o; eauto.
+  Qed.
+
+  Hint Resolve clean_ciphers_no_new_ciphers.
+
+  Lemma clean_ciphers_eliminates_added_dishonest_cipher :
+    forall c_id c cs k,
+      cs $? c_id = None
+      -> honest_keyb honestk k = false
+      -> k = cipher_signing_key c
+      -> clean_ciphers cs = clean_ciphers (cs $+ (c_id,c)).
+  Proof.
+    intros.
+    apply map_eq_Equal; unfold Equal; intros.
+    cases (y ==n c_id); subst.
+    - rewrite clean_ciphers_no_new_ciphers; auto.
+      symmetry.
+      eapply clean_ciphers_eliminates_dishonest_cipher; eauto.
+    - unfold clean_ciphers at 2, filter.
+      rewrite fold_add; auto. simpl.
+      unfold honest_cipher_filter_fn at 1.
+      cases c; simpl in *; rewrite H0; trivial.
+  Qed.
+
+  Lemma not_in_ciphers_not_in_cleaned_ciphers :
+    forall c_id cs,
+      ~ In c_id cs
+      -> ~ In c_id (clean_ciphers cs).
+  Proof.
+    intros.
+    rewrite not_find_in_iff in H.
+    apply not_find_in_iff; eauto.
+  Qed.
+
+  Hint Resolve not_in_ciphers_not_in_cleaned_ciphers.
+
+  Lemma dishonest_cipher_cleaned :
+    forall cs c_id cipherMsg,
+      honest_keyb honestk (cipher_signing_key cipherMsg) = false
+      -> ~ In c_id cs
+      -> clean_ciphers cs = clean_ciphers (cs $+ (c_id, cipherMsg)).
+  Proof.
+    intros.
+    apply map_eq_Equal; unfold Equal; intros.
+
+    case_eq (cs $? y); intros.
+
+    - eapply clean_ciphers_reduces_or_keeps_same_ciphers in H1.
+      destruct H1; destruct H1;
+        rewrite H1;
+        unfold clean_ciphers, filter;
+        rewrite fold_add by auto;
+        symmetry;
+        unfold honest_cipher_filter_fn; cases cipherMsg; simpl in *;
+          rewrite H; simpl; auto.
+
+    - rewrite clean_ciphers_no_new_ciphers; auto.
+      eapply clean_ciphers_no_new_ciphers in H1.
+      unfold clean_ciphers, filter. rewrite fold_add by auto.
+      unfold honest_cipher_filter_fn; cases cipherMsg; simpl in *; rewrite H; eauto.
+  Qed.
+
+  Hint Resolve dishonest_cipher_cleaned.
+
+  Hint Extern 1 (honest_cipher_filter_fn _ _ ?c = _) => unfold honest_cipher_filter_fn; cases c.
+
+  Lemma clean_ciphers_added_honest_cipher_not_cleaned :
+    forall cs c_id c k,
+      honest_key honestk k
+      -> k = cipher_signing_key c
+      -> clean_ciphers (cs $+ (c_id,c)) = clean_ciphers cs $+ (c_id,c).
+  Proof.
+    intros.
+    apply map_eq_Equal; unfold Equal; intros.
+
+    case (y ==n c_id); intros; subst; clean_map_lookups.
+    - erewrite clean_ciphers_keeps_honest_cipher; auto.
+      invert H; unfold honest_cipher_filter_fn; eauto.
+      unfold cipher_honestly_signed, honest_keyb;
+        cases c; simpl in *; context_map_rewrites; auto.
+    - case_eq (clean_ciphers cs $? y); intros; subst.
+      + cases (cs $? y); subst; eauto.
+        * assert (cs $? y = Some c1) by assumption;
+            eapply clean_ciphers_reduces_or_keeps_same_ciphers in Heq; split_ors;
+              split_ands; subst; contra_map_lookup.
+          eapply clean_ciphers_keeps_honest_cipher; auto.
+          unfold honest_cipher_filter_fn, cipher_honestly_signed;
+            cases c1; simpl in *; auto.
+        * exfalso; eapply clean_ciphers_no_new_ciphers in Heq; contra_map_lookup.
+      + case_eq (cs $? y); intros; subst; eauto.
+        eapply clean_ciphers_eliminates_dishonest_cipher; eauto.
+        case_eq (honest_keyb honestk (cipher_signing_key c0)); intros; subst; auto.
+        exfalso; eapply clean_ciphers_keeps_honest_cipher in H1; contra_map_lookup; auto.
+        unfold honest_cipher_filter_fn, cipher_honestly_signed;
+          cases c0; simpl in *; auto.
+  Qed.
+
+  Lemma clean_ciphers_idempotent :
+    forall cs,
+      ciphers_honestly_signed honestk cs
+      -> clean_ciphers cs = cs.
+  Proof.
+    unfold clean_ciphers, filter, ciphers_honestly_signed; intros.
+    apply P.fold_rec_bis; intros; Equal_eq; subst; eauto.
+    unfold honest_cipher_filter_fn.
+    rewrite find_mapsto_iff in H0.
+    assert (cipher_honestly_signed honestk e = true).
+    eapply Forall_natmap_in_prop with (P := fun c => cipher_honestly_signed honestk c = true); eauto.
+    rewrite H2; trivial.
+  Qed.
+
+  Lemma clean_ciphers_honestly_signed :
+    forall cs,
+      ciphers_honestly_signed honestk (clean_ciphers cs).
+  Proof.
+    unfold ciphers_honestly_signed; intros.
+    rewrite Forall_natmap_forall; intros.
+    rewrite <- find_mapsto_iff, clean_ciphers_mapsto_iff in H; split_ands.
+    unfold honest_cipher_filter_fn in *; assumption.
+  Qed.
+
+End CleanCiphers.
+
+(******************** MESSAGE CLEANING ********************
+ **********************************************************
+ *
+ * Function to clean messages and lemmas about it.
+ *)
+
+Section CleanMessages.
+  Import RealWorld.
+
+  Section CleanMessagesImpl.
+    Variable honestk : key_perms.
+    Variable msgs : queued_messages.
+
+    Definition msg_filter (sigM : { t & message t } ) : bool :=
+      match sigM with
+      | existT _ _ msg => msg_honestly_signed honestk msg
+      end.
+
+    Definition clean_messages :=
+      List.filter msg_filter.
+
+  End CleanMessagesImpl.
+
+  Lemma clean_messages_keeps_honestly_signed :
+    forall {t} (msg : message t) honestk msgs,
+      msg_honestly_signed honestk msg = true
+      -> clean_messages honestk (msgs ++ [existT _ _ msg])
+        = clean_messages honestk msgs ++ [existT _ _ msg].
+  Proof.
+    intros; unfold clean_messages.
+    induction msgs; simpl; eauto.
+    - rewrite H; trivial.
+    - cases (msg_filter honestk a); subst; eauto.
+      rewrite IHmsgs; trivial.
+  Qed.
+
+  Lemma clean_messages_drops_not_honestly_signed :
+    forall {t} (msg : message t) msgs honestk,
+      msg_honestly_signed honestk msg = false
+      -> clean_messages honestk (msgs ++ [existT _ _ msg])
+        = clean_messages honestk msgs.
+  Proof.
+    intros; unfold clean_messages.
+    induction msgs; simpl; eauto.
+    - rewrite H; trivial.
+    - cases (msg_filter honestk a); subst; eauto.
+      rewrite IHmsgs; trivial.
+  Qed.
+
+  Lemma clean_message_keeps_safely_patterned_message :
+    forall {t} (msg : message t) honestk msgs pat,
+      msg_pattern_safe honestk pat
+      -> msg_accepted_by_pattern pat msg
+      -> clean_messages honestk (existT _ _ msg :: msgs)
+        = (existT _ _ msg) :: clean_messages honestk msgs.
+  Proof.
+    intros.
+    assert (msg_honestly_signed honestk msg = true) by eauto.
+    unfold clean_messages; simpl;
+      match goal with
+      | [ H : msg_honestly_signed _ _ = _ |- _ ] => rewrite H
+      end; trivial.
+  Qed.
+
+  Lemma clean_messages_idempotent :
+    forall msgs honestk,
+      clean_messages honestk (clean_messages honestk msgs) = clean_messages honestk msgs.
+  Proof.
+    induction msgs; intros; eauto.
+    simpl.
+    case_eq (msg_filter honestk a); intros; eauto.
+    simpl; rewrite H; auto.
+    rewrite IHmsgs; trivial.
+  Qed.
+
+End CleanMessages.
+
+(******************** USER CLEANING ***********************
+ **********************************************************
+ *
+ * Function to clean users and lemmas about it.
+ *)
+
+Section CleanUsers.
+  Import RealWorld.
+
+  Variable honestk : key_perms.
+
+  Definition clean_users {A} (usrs : honest_users A) :=
+    map (fun u_d => {| key_heap := u_d.(key_heap)
+                  ; protocol := u_d.(protocol)
+                  ; msg_heap := clean_messages honestk u_d.(msg_heap)
+                  ; c_heap   := u_d.(c_heap) |}) usrs.
+
+  Lemma clean_users_cleans_user :
+    forall {A} (usrs : honest_users A) u_id u_d u_d',
+      usrs $? u_id = Some u_d
+      -> u_d' = {| key_heap := u_d.(key_heap)
+                ; protocol := u_d.(protocol)
+                ; msg_heap :=  clean_messages honestk u_d.(msg_heap)
+                ; c_heap   := u_d.(c_heap) |}
+      -> clean_users usrs $? u_id = Some u_d'.
+  Proof.
+    intros.
+    unfold clean_users; rewrite map_o; unfold option_map;
+      context_map_rewrites; subst; auto.
+  Qed.
+
+  Lemma clean_users_cleans_user_inv :
+    forall {A} (usrs : honest_users A) u_id u_d,
+      clean_users usrs $? u_id = Some u_d
+      -> exists msgs, usrs $? u_id = Some {| key_heap := u_d.(key_heap)
+                                     ; protocol := u_d.(protocol)
+                                     ; msg_heap := msgs
+                                     ; c_heap   := u_d.(c_heap) |}
+                /\ u_d.(msg_heap) = clean_messages honestk msgs.
+  Proof.
+    intros.
+    unfold clean_users in *. rewrite map_o in H. unfold option_map in *.
+    cases (usrs $? u_id); try discriminate; eauto.
+    destruct u; destruct u_d; simpl in *.
+    invert H.
+    eexists; eauto.
+  Qed.
+
+  Lemma clean_users_add_pull :
+    forall {A} (usrs : honest_users A) u_id u,
+      clean_users (usrs $+ (u_id,u))
+      = clean_users usrs $+ (u_id, {| key_heap := u.(key_heap)
+                                    ; protocol := u.(protocol)
+                                    ; msg_heap :=  clean_messages honestk u.(msg_heap)
+                                    ; c_heap   := u.(c_heap) |}).
+  Proof.
+    intros.
+    apply map_eq_Equal; unfold Equal; intros.
+    cases (y ==n u_id); subst; clean_map_lookups; eauto;
+      unfold clean_users; rewrite !map_o; unfold option_map; clean_map_lookups; auto.
+  Qed.
+
+  Hint Resolve findUserKeys_foldfn_proper findUserKeys_foldfn_transpose
+       findUserKeys_foldfn_proper_Equal findUserKeys_foldfn_transpose_Equal.
+
+  Lemma clean_users_no_change_findUserKeys :
+    forall {A} (usrs : honest_users A),
+      findUserKeys (clean_users usrs) = findUserKeys usrs.
+  Proof.
+    induction usrs using P.map_induction_bis; intros; Equal_eq; contra_map_lookup; auto.
+    unfold findUserKeys.
+    rewrite fold_add; auto.
+    rewrite clean_users_add_pull; auto. simpl.
+    apply map_eq_Equal; unfold Equal; intros.
+    rewrite !fold_add; auto. simpl.
+    rewrite !findUserKeys_notation, IHusrs; trivial.
+
+    unfold not; intros.
+    apply map_in_iff in H0; contradiction.
+  Qed.
+
+  Lemma clean_users_idempotent :
+    forall {A} (usrs : honest_users A),
+      clean_users (clean_users usrs) = clean_users usrs.
+  Proof.
+    intros; apply map_eq_Equal; unfold Equal; intros.
+    case_eq (clean_users usrs $? y); intros.
+    - destruct u; simpl in *; eapply clean_users_cleans_user; eauto; simpl.
+      apply clean_users_cleans_user_inv in H.
+      destruct H; split_ands; simpl in *; eauto.
+      f_equal; subst; eauto using clean_messages_idempotent.
+    - unfold clean_users in *.
+      rewrite map_o in H; unfold option_map in H; cases (usrs $? y); try discriminate.
+
+      rewrite !map_o, Heq; trivial.
+  Qed.
+
+End CleanUsers.
+
+Section StripAdv.
+  Import RealWorld.
+
+  Definition strip_adversary {A B} (U__r : universe A B) (b : B) : universe A B :=
+    let honestk := findUserKeys U__r.(users)
+    in {| users       := clean_users honestk U__r.(users)
+        ; adversary   := {| key_heap := U__r.(adversary).(key_heap)
+                          ; msg_heap := U__r.(adversary).(msg_heap)
+                          ; protocol := Return b
+                          ; c_heap   := U__r.(adversary).(c_heap) |}
+        ; all_ciphers := clean_ciphers honestk U__r.(all_ciphers)
+        ; all_keys    := U__r.(all_keys)
+       |}.
+End StripAdv.
